Prove a few facts about identity
Signed-off-by: Nicolas Iooss <nicolas.iooss_git@polytechnique.org>

identity.v
@@ -1,5 +1,5 @@
 (** Example of function: the identity *)
-Require Import compiler free_variables krivine lterm.
+Require Import beta_reduction compiler compiler_correct free_variables krivine lterm.
 
 Definition l_id: lterm := Lambda (Var O)
 .
@@ -7,9 +7,8 @@ Definition l_id: lterm := Lambda (Var O)
 Definition krivine_id : krivine_code := Grab (Access 0 Nop)
 .
 
-
 (** Identity is closed *)
-Lemma closed_id:
+Theorem closed_id:
   closed l_id.
 Proof.
   unfold closed.
@@ -19,7 +18,7 @@ Proof.
 Save.
 
 (** Compilation *)
-Lemma compile_id:
+Theorem compile_id:
   comp l_id = krivine_id.
 Proof.
   unfold l_id.
@@ -28,10 +27,36 @@ Proof.
 Save.
 
 (** Reverse compilation *)
-Lemma tau_id:
+Theorem tau_id:
   tau_code krivine_id = Some l_id.
 Proof.
   unfold l_id.
   unfold krivine_id.
+  trivial.
+Save.
+
+(** Correct state *)
+Definition kstate_id : krivine_env := krivine_state krivine_id KEnv_nil KEnv_nil
+.
+
+Theorem correct_id:
+  correct_state kstate_id.
+Proof.
+  apply correct_env_is_state.
+  apply Correct_env; simpl.
+    unfold closed_code.
+    exists l_id.
+    elim tau_id.
+    apply conj; trivial.
+    apply closed_id.
+  apply Correct_env_nil.
+  apply Correct_env_nil.
+Save.
+
+(** Identity is a final state in krivine machine *)
+Theorem final_step:
+  krivine_step kstate_id = kstate_id.
+Proof.
+  unfold kstate_id.
   trivial.
 Save.
