Makefile
@@ -31,7 +31,7 @@ beta_reduction.vo: lterm.vo substitution.vo
 compiler_correct.vo: beta_reduction.vo compiler.vo krivine.vo lterm.vo substitute_list.vo
 compiler.vo: free_variables.vo krivine.vo lterm.vo substitute_list.vo
 free_variables.vo: Arith_ext.vo lterm.vo
-identity.vo: compiler.vo free_variables.vo krivine.vo lterm.vo
+identity.vo: beta_reduction.vo compiler.vo compiler_correct.vo free_variables.vo krivine.vo lterm.vo
 substitute_list.vo: Arith_ext.vo free_variables.vo lterm.vo substitute_varlist.vo
 substitute_varlist.vo: Arith_ext.vo lterm.vo substitution.vo
 substitution.vo: Arith_ext.vo free_variables.vo lterm.vo
